imper/MutableList.ml
@@ -1,60 +1,41 @@
 open NullPointers
 
-type 'a mlist = ('a * 'a mlist) ref 
+type 'a mlist = { mutable hd : 'a ; 
+                  mutable tl : 'a mlist }
 
-let is_nil (l:'a mlist) =
-   l == null
-
-let head (l:'a mlist) =
-   fst (!l)
-
-let tail (l:'a mlist) =
-   snd (!l)
-
-let set_head (l:'a mlist) x =
-   let (_,t) = !l in
-   l := (x,t)
-
-let set_tail (l:'a mlist) t =
-   let (x,_) = !l in
-   l := (x,t)
-
-let append (l1 : 'a mlist) (l2 : 'a mlist) =
-   if l1 == null then l2 else
-   let h = ref l1 in
-   while not (is_nil (tail (!h))) do
-      h := tail (!h);
-   done;
-   set_tail (!h) l2;
-   l1
    
 let length (l:'a mlist) =
    let h = ref l in
    let n = ref 0 in
-   while not (is_nil (!h)) do
+   while !h != null do
      incr n;
-     h := tail !h;
+     h := !h.tl;
    done;
    !n
 
-(*--todo: needs to be fixed
-    so as to avoid reallocating cells 
-let rev (l:'a mlist) =
+let append (l1 : 'a mlist) (l2 : 'a mlist) =
+   if l1 == null then l2 else
+   let h = ref l1 in
+   while !h.tl != null do
+      h := !h.tl;
+   done;
+   !h.tl <- l2;
+   l1
+
+let inplace_rev (l:'a mlist) =
   let f = ref l in
   let r = ref (null:'a mlist) in
   while !f != null do
-    let ((x:'a),t) = !(!f) in
-    r := ref (x, !r);
-    f := t;
+    let c = !f in
+    let n = c.tl in
+    c.tl <- !r;
+    r := c;
+    f := n;
   done;
   !r
-*)
 
+let rec cps_append (x:'a mlist) (y:'a mlist) (k:'a mlist->'b) : 'b =
+  if x == null then k y else
+    let f z = (x.tl <- z; k x) in 
+    cps_append x.tl y f
 
-(* test
-let _ =
-  let x = ref (3, ref (5, null)) in
-  Printf.printf "%d\n" (length x)
-*)
-(* 
-*)
