imper/MutableList_proof.v
@@ -1,9 +1,9 @@
 Set Implicit Arguments.
-Require Import LibCore CFPrim MutableList_ml LibList.
+Require Import LibCore CFLib MutableList_ml LibList.
 Module ML := MutableList_ml.
 Opaque MList Ref MListSeg.
 
-(*todo:remove*)
+(*todo:remove
 Ltac xapps_core spec args solver ::=
   let cont1 tt :=
     xapp_with spec args solver in
@@ -13,53 +13,227 @@ Ltac xapps_core spec args solver ::=
   | tag_let_trm => xlet; [ cont1 tt | cont2 tt ]
   | tag_seq =>     xseq; [ cont1 tt | cont2 tt ]
   end.
+*)
+
+
+Lemma himpl_extens : forall H1 H2 : hprop,
+  H1 ==> H2 -> H2 ==> H1 -> H1 = H2.
+Proof. intros. unfold hprop. extens*. Qed.
+
+Lemma himpl_proj1 : forall H1 H2 : hprop,
+  H1 = H2 -> H1 ==> H2.
+Proof. intros. subst~. Qed.
+
+Lemma himpl_proj2 : forall H1 H2 : hprop,
+  H1 = H2 -> H2 ==> H1.
+Proof. intros. subst~. Qed.
+(*
+Lemma himpl_id : forall H1 H2 : hprop,
+  H1 ==> H2 -> H1 ==> H2.
+Proof. auto. Qed.
+Implicit Arguments himpl_id [H1 H2].
+*)
+
+Implicit Arguments himpl_proj1 [H1 H2].
+Implicit Arguments himpl_proj2 [H1 H2].
+Implicit Arguments himpl_extens [H1 H2].
+
+
+Ltac hchange_apply L cont :=
+  eapply hchange_lemma; 
+    [ apply L | cont tt | ].
+
+Ltac hchange_forwards L modif cont :=
+  let K := fresh "TEMP" in
+  forwards_nounfold K: L; 
+  match modif with
+  | __ => hchange_apply K cont
+  | _ => hchange_apply (@modif _ _ K) cont
+  end; clear K.
+
+Ltac hchange_core E modif :=
+  match E with
+(*  | ?H ==> ?H' => hchange_with_core H H' *)
+  | _ => hchange_forwards E modif ltac:(fun _ => instantiate; hsimpl)
+  end.
+
+Tactic Notation "hchange_debug" constr(E) :=
+  hchange_forwards E __ ltac:(idcont).
+Tactic Notation "hchange_debug" "->" constr(E) :=
+  hchange_forwards E himpl_proj1 ltac:(idcont).
+Tactic Notation "hchange_debug" "<-" constr(E) :=
+  hchange_forwards himpl_proj2 ltac:(idcont).
+
+Tactic Notation "hchange" constr(E) :=
+  hchange_core E __.
+Tactic Notation "hchange" "->" constr(E) :=
+  hchange_core E himpl_proj1.
+Tactic Notation "hchange" "<-" constr(E) :=
+  hchange_core E himpl_proj2.
+
+
+Tactic Notation "hchange" "~" constr(E) :=
+  hchange E; auto~.
+Tactic Notation "hchange" "*" constr(E) :=
+  hchange E; auto*.
+
+
+
+
+
+
+
+Ltac xchange_apply L cont :=
+   eapply xchange_lemma; 
+     [ try xlocal | apply L | cont tt | ].
+
+(* note: modif should be himpl_proj1 or himpl_proj2 *)
+Ltac xchange_forwards L modif cont :=
+  let K := fresh "TEMP" in
+  forwards_nounfold K: L; 
+  match modif with
+  | __ => xchange_apply K cont
+  | _ => xchange_apply (@modif _ _ K) cont
+  end; clear K.
+
+Ltac xchange_with H H' :=
+  eapply xchange_lemma with (H1:=H) (H1':=H'); 
+    [ try xlocal | | hsimpl | ].
+
+Ltac xchange_core E modif :=
+  match E with
+  | ?H ==> ?H' => xchange_with_core H H'
+  | _ => xchange_forwards E modif ltac:(fun _ => instantiate; hsimpl)
+  end.
+
+Tactic Notation "xchange_debug" constr(E) :=
+  xchange_forwards E __ ltac:(idcont).
+Tactic Notation "xchange_debug" "->" constr(E) :=
+  xchange_forwards E himpl_proj1 ltac:(idcont).
+Tactic Notation "xchange_debug" "<-" constr(E) :=
+  xchange_forwards himpl_proj2 ltac:(idcont).
+
+Tactic Notation "xchange" constr(E) :=
+  xchange_core E __.
+Tactic Notation "xchange" "->" constr(E) :=
+  xchange_core E himpl_proj1.
+Tactic Notation "xchange" "<-" constr(E) :=
+  xchange_core E himpl_proj2.
+
+
+Tactic Notation "xchange" "~" constr(E) :=
+  xchange E; auto~.
+
+
+Lemma heap_is_single_null_eq_false : forall A (v:A),
+  heap_is_single null v = [False].
+Proof. intros.  Transparent heap_is_empty_st heap_is_single. unfold heap_is_single.
+ unfold hprop. extens. intros. unfold heap_is_empty_st. auto*.
+Opaque heap_is_single heap_is_empty_st.
+Qed.
+
+Lemma heap_is_single_null_to_false : forall A (v:A),
+  heap_is_single null v ==> [False].
+Proof. introv Hh. forwards*: heap_is_single_null. Qed. 
 
 
 (********************************************************************)
-(* ** Accessors *)
+(* ** Representation predicate for mutable lists *)
 
-Lemma is_nil_spec : forall a,
-  Spec is_nil (l:mlist a) |R>> forall A (T:A->a->hprop) (L:list A),
-     keep R (l ~> MList T L) (\[ bool_of (L = nil) ]).
+Fixpoint MList A a (T:A->a->hprop) (L:list A) (l:loc) : hprop :=
+  match L with
+  | nil => [l = null]
+  | X::L' => l ~> Mlist T (MList T) X L'
+  end.
+
+Section MListProp.
+Variables (A a : Type) (T:A->a->hprop).
+
+Lemma MList_nil : forall l,
+  l ~> MList T nil = [l = null].
+Proof. intros. hdata_simpl Mlist. auto. Qed.
+
+Lemma MList_cons : forall l X L',
+  l ~> MList T (X::L') = 
+  Hexists x l', l ~> Mlist Id Id x l' \* x ~> T X \* l' ~> MList T L'.
+Proof. intros. simpl. hdata_simpl. rewrite~ Mlist_convert. Qed.
+
+Lemma MList_null : forall L,
+  null ~> MList T L = [L = nil].
 Proof.
-  xcf. intros. xapp. intros b. hextract.
-  hchange (unfocus_mnil'' l). hextract. subst b. hsimpl. xclean. iff*.
-Qed.
+  intros. destruct L; simpl; hdata_simpl.
+  apply himpl_extens; xsimpl~.
+  apply himpl_extens.
+    unfold Mlist. hdata_simpl. hextract. 
+     rewrite heap_is_single_null_eq_false. hextract. false.
+    hextract. false.
+Qed.  
 
-Lemma head_spec : forall a,
-  Spec ML.head (l:mlist a) |R>> forall (x:a) (t:mlist a),
-    keep R (l ~> Ref Id (x,t)) (\= x).
-Proof. 
-  xcf. intros. xapps. xret.
-Qed.
-
-Lemma tail_spec : forall a,
-  Spec ML.tail (l:mlist a) |R>> forall (x:a) (t:mlist a),
-    keep R (l ~> Ref Id (x,t)) (\= t).
-Proof. 
-  xcf. intros. xapps. xret.
-Qed.
-
-Lemma set_head_spec : forall a,
-  Spec ML.set_head (l:mlist a) (x:a) |R>> forall (x':a) (t:mlist a),
-    R (l ~> Ref Id (x',t)) (# l ~> Ref Id (x,t)).
-Proof. 
-  xcf. intros. xapps. xmatch. xapp. hsimpl.
-Qed.
-
-Lemma set_tail_spec : forall a,
-  Spec ML.set_tail (l:mlist a) (t:mlist a) |R>> forall (x:a) (t':mlist a),
-    R (l ~> Ref Id (x,t')) (# l ~> Ref Id (x,t)).
-Proof. 
-  xcf. intros. xapps. xmatch. xapp. hsimpl.
+Lemma MList_not_null : forall l L,
+  l <> null -> 
+  l ~> MList T L ==> l ~> MList T L \* [L <> nil].
+Proof.
+  intros. destruct L.
+  hchange -> (MList_nil l). hextract. false.
+  hsimpl. auto_false.
 Qed.
 
 
-Hint Extern 1 (RegisterSpec is_nil) => Provide is_nil_spec.
-Hint Extern 1 (RegisterSpec ML.head) => Provide head_spec.
-Hint Extern 1 (RegisterSpec ML.tail) => Provide tail_spec.
-Hint Extern 1 (RegisterSpec ML.set_head) => Provide set_head_spec.
-Hint Extern 1 (RegisterSpec ML.set_tail) => Provide set_tail_spec.
+
+
+(*------------------------------------------------------------------*)
+(* ** MLists *)
+
+
+Lemma focus_mnil : forall A a (T:A->a->hprop),
+  [] ==> null ~> MList T nil.
+Proof. intros. simpl. hdata_simpl. hsimpl~. Qed.
+
+Lemma unfocus_mnil : forall (l:loc) A a (T:A->a->hprop),
+  l ~> MList T nil ==> [l = null].
+Proof. intros. simpl. hdata_simpl. hsimpl~. Qed.
+
+Lemma unfocus_mnil' : forall A (L:list A) a (T:A->a->hprop),
+  null ~> MList T L ==> [L = nil].
+Proof.
+  intros. destruct L.
+  simpl. unfold hdata. hextract. hsimpl~. 
+  unfold hdata, MList. hchange focus_ref2_null. hextract. false.
+Qed.
+
+Lemma unfocus_mnil'' : forall (l:loc) A (L:list A) a (T:A->a->hprop),
+  l ~> MList T L ==> [l = null <-> L = nil] \* l ~> MList T L.
+Proof. skip. (*todo*) Qed.
+
+Lemma focus_mcons : forall (l:loc) a A (X:A) (L':list A) (T:A->a->hprop),
+  (l ~> MList T (X::L')) ==>
+  Hexists x l', (x ~> T X) \* (l' ~> MList T L') \* (l ~> Ref Id (x,l')).
+Proof.
+  intros. simpl. hdata_simpl. hchange (@focus_ref2 l). hextract. hsimpl.
+Qed.
+
+Lemma focus_mcons' : forall (l:loc) a A (L:list A) (T:A->a->hprop),
+  [l <> null] \* (l ~> MList T L) ==> 
+  Hexists x l', Hexists X L', 
+    [L = X::L'] \*  (l ~> Ref Id (x,l')) \* (x ~> T X) \* (l' ~> MList T L').
+Proof.
+  intros. destruct L. lets: (@unfocus_mnil l _ _ T). (* Show Existentials. *)
+  hextract. false~.
+  hchange (@focus_mcons l). hextract as x l' E. hsimpl~.  
+Qed.
+
+Lemma unfocus_mcons : forall (l:loc) a (x:a) (l':loc) A (X:A) (L':list A) (T:A->a->hprop),
+  (l ~> Ref Id (x,l')) \* (x ~> T X) \* (l' ~> MList T L') ==> 
+  (l ~> MList T (X::L')).
+Proof.
+  intros. simpl. hdata_simpl. hchange (@unfocus_ref2 l _ x _ l'). hsimpl.
+Qed.
+
+Global Opaque MList.
+
+Implicit Arguments unfocus_mnil [ ].
+Implicit Arguments unfocus_mcons [ a A ].
+Implicit Arguments focus_mcons [ a A ].
 
 
 
