Makefile
@@ -100,20 +100,8 @@ VAC=\
 	vacid/sparse_array_proof.v 
 
 NEW=\
-	imper/CPS_ml.v \
-	imper/CPS_proof.v \
-	demo/test_ml.v \
-	demo/test_proof.v \
-	imper/ListIterators_ml.v \
-	imper/ListIterators_proof.v \
-	imper/LambdaEval_ml.v \
-	imper/LambdaEval_proof.v \
-	imper/Compose_ml.v \
-	imper/Compose_proof.v \
-	imper/Swap_ml.v \
-	imper/Swap_proof.v \
-	imper/TreeCopy_ml.v \
-	imper/TreeCopy_proof.v \
+	imper/MutableList_ml.v \
+	imper/MutableList_proof.v 
 
 IMP=\
 	CFHeaps.v \
@@ -128,21 +116,32 @@ IMPER=\
 	imper/Landin_proof.v \
 	imper/Counter_ml.v \
 	imper/Facto_ml.v \
-	imper/MutableList_ml.v \
 	imper/TreeCopy_ml.v \
 	imper/Loops_ml.v \
 	imper/StrongUpdate_ml.v \
 	imper/InOut_ml.v \
 	imper/Counter_proof.v \
 	imper/Facto_proof.v \
-	imper/MutableList_proof.v \
 	imper/TreeCopy_proof.v \
 	imper/Loops_proof.v \
 	imper/StrongUpdate_proof.v \
 	imper/InOut_proof.v \
 	imper/Dijkstra_ml.v \
-	imper/Dijkstra_proof.v 
-
+	imper/Dijkstra_proof.v  \
+	imper/CPS_ml.v \
+	imper/CPS_proof.v \
+	demo/test_ml.v \
+	demo/test_proof.v \
+	imper/ListIterators_ml.v \
+	imper/ListIterators_proof.v \
+	imper/LambdaEval_ml.v \
+	imper/LambdaEval_proof.v \
+	imper/Compose_ml.v \
+	imper/Compose_proof.v \
+	imper/Swap_ml.v \
+	imper/Swap_proof.v \
+	imper/TreeCopy_ml.v \
+	imper/TreeCopy_proof.v 
 
 #	okasaki/Okasaki_ml.v
 
